\documentclass{article}

\usepackage{amsmath}
\usepackage{forest} % tree
\usepackage{geometry} % page layout
\geometry{
    left=3cm,
    right=3cm,
}

\begin{document}

\title{Homework 2}
\author{Pupipat Singkhorn}
\date{\today}
\maketitle

\section*{Exercise 2}

\begin{enumerate}
    \item Consider the context-free grammar:
    \[
    S \rightarrow S S + \mid S S^* \mid a
    \]
    and the string $aa + a^*$.
    \begin{enumerate}
        \item Give a leftmost derivation for the string.
        \\ $ S \rightarrow SS^* $
        \\ $ \rightarrow SS + S^* $
        \\ $ \rightarrow aS + S^* $
        \\ $ \rightarrow aa + S^* $
        \\ $ \rightarrow aa + a^* $
        \item Give a rightmost derivation for the string.
        \\ $ S \rightarrow SS^* $
        \\ $ \rightarrow Sa^* $
        \\ $ \rightarrow SS + a^* $
        \\ $ \rightarrow aS + a^* $
        \\ $ \rightarrow aa + a^* $
        \item Give a parse tree for the string.\\
        \begin{forest}
            [S
                [S
                    [S [a]]
                    [S [a]]
                    [+]
                ]
                [S
                    [a]
                ]
                [*]
            ]
            \end{forest}
        \item Is the grammar ambiguous or unambiguous? Justify your answer.
        \\ : Unambiguous, leftmost and rightmost generate the same parse tree.
    \end{enumerate}
    \newpage
    \item Consider the context-free grammar:
    \[
    S \rightarrow S + S \mid S S \mid (S) \mid S^* \mid a
    \]
    and the string $(a+a)^*a$.
    \begin{enumerate}
        \item Give a leftmost derivation for the string.
        \\ $ S \rightarrow SS $
        \\ $ \rightarrow S^* S $
        \\ $ \rightarrow (S)^* S $
        \\ $ \rightarrow (S+S)^* S $
        \\ $ \rightarrow (a+S)^* S $
        \\ $ \rightarrow (a+a)^* S $
        \\ $ \rightarrow (a+a)^* a $
        \item Give a rightmost derivation for the string.
        \\ $ S \rightarrow SS $
        \\ $ \rightarrow Sa $
        \\ $ \rightarrow S^* a $
        \\ $ \rightarrow (S)^* a $
        \\ $ \rightarrow (S+S)^* a $
        \\ $ \rightarrow (S+a)^* a $
        \\ $ \rightarrow (a+a)^* a $
        \item Give a parse tree for the string.\\
        \begin{forest}
            [S
                [S
                    [S
                        [(]
                        [S
                            [S [a]]
                            [+]
                            [S [a]]
                        ]
                        [)]
                    ]
                    [*]
                ]
                [S [a]]
            ]
        \end{forest}
        \item Is the grammar ambiguous or unambiguous? Justify your answer.
        \\ : Ambiguous, the string `aaa' can be generated by two different parse trees.\\
        \begin{center}
            \begin{forest}
                [S
                    [S [a]]
                    [S
                        [S [a]]
                        [S [a]]
                    ]
                ]
            \end{forest}
            \hspace{5em}
            \begin{forest}
                [S
                    [S
                        [S [a]]
                        [S [a]]
                    ]
                    [S [a]]
                ]
            \end{forest}
        \end{center}
    \end{enumerate}

    \item Design grammars for the following languages:
    \begin{enumerate}
        \item The set of all strings of 0s and 1s such that every 0 is immediately followed by \\at least one 1.
        \\ $ S \rightarrow AB $
        \\ $ A \rightarrow 1A \mid \lambda $
        \\ $ B \rightarrow CB \mid \lambda $
        \\ $ C \rightarrow 01A $
        \item The set of all strings of 0s and 1s that are palindromes; that is, the string reads the same backward as forward.
        \\ $ S \rightarrow 0S0 \mid 1S1 \mid 0 \mid 1 \mid \lambda $
        \item The set of all strings of 0s and 1s with an equal number of 0s and 1s.
        \\ $ S \rightarrow 0S1S \mid 1S0S \mid \lambda $
        \item The set of all strings of 0s and 1s in which 011 does not appear as a substring.
        \\ $ S \rightarrow ABCB $
        \\ $ A \rightarrow 1A \mid \lambda $
        \\ $ B \rightarrow 0B \mid \lambda $
        \\ $ C \rightarrow 01C \mid \lambda $
    \end{enumerate}
\end{enumerate}

\end{document}
